---
Source:
  - https://youtube.com/watch?v=byiJ4sW2ZPY
Reviewed: false
---
- Difference of squares
	- $A^2 - B^2 = (A + B) (A - B)$ 
- Perfect Square
	- $A^2 + 2AB + B^2 = (A+B)^2$ 
		- First term is squared
		- Second term is twice the product of both terms
		- Last term is squared
	- $A^2 - 2AB + B^2 = (A-B)^2$ 
- Sum of cubes
	- $A^3 + B^3 = (A + B) (A^2 - AB + B^2)$ 
- Difference of cubes
	- $A^3 - B^3 = (A - B) (A^2 + AB + B^2)$ 
- ![[Screenshot 2023-01-21 at 9.14.00 PM.png]]
	- Some Special Considerations
		- (1) Factoring out common factors first
		- (2) Substitute
		- (3) [[(8) PreCalculus - Algebra Fundamental Review (7 of 80) Factoring - Examples|Special technique]] (2 middle terms)