---
aliases: exponents
explored:
---
## Synthesis
- 
## Source [^1]
### Properties
- (1) $a^ma^n = a^{m+n}$
	- $a^2a^3 = a^{2+3} = a^5$
- (2) $\frac {a^m}{a^n} = a^{m-n}$
	- $\frac {a^4}{a^2} = a^{4-2} = a^2$ 
- (3) $a^0 = 1$
	- $\frac {a^3}{a^3} = \frac{aaa}{aaa} = 1$
- (4) $a^{-m} = \frac {1}{a^m}$
	- $\frac {a^2}{a^4} = a^{2-4} = a^{-2} = \frac {1}{a^2}$
- (5) $(a^m)^n = a^{m*n}$ 
	- $(a^3)^2 = a^{3*2} = a^6$
	- Parenthesis are important! [^2]
		- $a^{m^n} \ne (a^m)^n$
- (6) $(ab)^m = a^mb^m$ 
	- $(ab)^3 = a^3b^3$
- (7) $(\frac {a}{b})^m = \frac {a^m}{b^m}$ 
	- $(\frac {a}{b})^3 = \frac {a^3}{b^3}$ 
- (8) $(\frac{a}{b})^{-m} = \frac{b^m}{a^m}$
	- $(\frac{a}{b})^{-2} = (\frac{b}{a})^2 = \frac{b^2}{a^2}$
- (9) $\sqrt[m]{a^n} = a^{\frac nm}$
	- $\sqrt[3]{8^2} = 4$
## Source[^3]
### Exponent odd or even
- Given $(-b)^x$
	- If power is even, answer is positive
	- If power is odd, answer is negative
- Examples
	- $(-1)^{24}$ = 1
	- $(-1)^{53}$ = -1
## Source[^4]
- Inverse of an exponential function is a logarithmic function
## References
[^1]: [[(1) PreCalc 1.1 Exponents]]
[^2]: [[Home Page - Building Blocks for Theoretical Computer Science by Margaret M. Fleck#^wjg58a]]
[^3]: https://content.byui.edu/file/b8b83119-9acc-4a7b-bc84-efacf9043998/1/Math-1-10-6.html#:~:text=The%20basic%20rule%20when%20a,%E2%86%92%20the%20answer%20is%20negative.
[^4]: https://web.ics.purdue.edu/~pdevlin/Traditional%20Class/Lesson%2032/Finding%20the%20Inverse%20of%20an%20Exponential%20or%20Logarithmic%20Function.pdf
