## Synthesis
- 
## Source [^1]
- A differential equation which can be written in the form $y^{\prime}+f(x) y=$ $g(x) y^{n}$. The transformation $z=y^{1-n}$ gives $z^{\prime}=\frac{d z}{d x}=(1-n) y^{-n} y^{\prime}$. Dividing the original equation by $y^{n}$ gives $y^{-n} y^{\prime}+f(x) y^{1-n}=g(x)$ which reduces to $\frac{1}{1-n} z^{\prime}+f(x) z=g(x)$ which is in linear form and can be solved by use of an integrating factor.
## References

[^1]: [[Home Page - The Concise Oxford Dictionary of Mathematics 6th Edition by Oxford Reference]]