## Synthesis
- 
## Source[^1]
- For n $\in$ $\mathbb{N}$
	- $(x+y)^n$ = $\Sigma_{k=0}^n$ $n \choose k$ $x^ky^{n-k}$ 

## Source[^2]
- A generalization of formulae such as $(x+y)^{2}=x^{2}+2 x y+y^{2}$ and $(x+y)^{3}=x^{3}+3 x^{2} y+3 x y^{2}+y^{3}$ used in elementary algebra. The Binomial Theorem states: for all positive integers $n$,$$

\begin{aligned}

& (x+y)^{n}=\sum_{r=0}^{n}\binom{n}{r} x^{n-r} y^{r} \\

& =x^{n}+\binom{n}{1} x^{n-1} y+\binom{n}{2} x^{n-2} y^{2}+\cdots+\binom{n}{r} x^{n-r} y^{r}+\cdots+y^{n}

\end{aligned}

$$where $\binom{n}{r}=\frac{n!}{r!(n-r)!}$ (see BINOMIAL COEFFICIENT).
- When $y=1$, the theorem agrees with the terminating binomial series. There is a multinomial theorem for more general expansions such as $\left(x_{1}+x_{2}+\cdots x_{k}\right)^{n}$.
## References

[^1]: [[(10) Counting Subsets and the Binomial Theorem (full lecture)]]
[^2]: [[Home Page - The Concise Oxford Dictionary of Mathematics 6th Edition by Oxford Reference]]