---
aliases:
  - completing the square
---
## Synthesis
- 
## Source[^1]
### Example
$$   
\begin{align*}  
4x^2 + 8x - 9 &= 0 &\text{Given}
\\ x^2 + 2x - \frac 94 &= 0 &\text{Divide by 4 (leading coefficient = 1)}
\\ \textcolor{hotpink}{(x + \frac 22)^2} - \frac 94 \textcolor{hotpink}{-(\frac 22)^2} &= 0 &\text{Complete the Square}
\\ (x+1)^2 - \frac {13}{4} &=0 &\text{Simplify}
\\ x + 1 &= \sqrt{\frac {13}{4}} &\text{Add and Square Root}
\\x &= -1 \pm \frac {\sqrt{13}}{2} &\text{Subtract}
\end{align*}  
$$
## References

[^1]: [[(Video) Algebra 1 Final Review (Part 2) - Factoring, Quadratic Formula, Graphing, Word Problems + More! by Ludus#^f67d80]]