## Synthesis
- 
## Source[^1]
- The converse and inverse are logically equivalent

### Examples
- Given the conditional $p \to q$, the converse would be $q \to p$
### Proof

#### Converse and Inverse Logically Equivalent

| p   | q   | $\lnot$p | $\lnot{q}$ | $p \implies q$ | $q \implies p$ | $\lnot{p} \implies \lnot {q}$ | $\lnot{q} \implies \lnot{p}$ |
| --- | --- | -------- | ---------- | -------------- | -------------- | ----------------------------- | ---------------------------- |
| T   | T   | F        | F          | T              | T              | T                             | T                            |
| T   | F   | F        | T          | F              | T              | T                             | F                            |
| F   | T   | T        | F          | T              | F              | F                             | T                            |
| F   | F   | T        | T          | T              | T              | T                             | T                            |
|     |     |          |            | Conditional    | Converse       | Inverse                       | Contrapositive               |

![[Screenshot 2023-05-12 at 10.06.13 AM.png|500]]
- Truth table shows that the [[converse]] and [[inverse]] of an [[Implication]] are logically equivalent
## References

[^1]: [[(15) The Conditional and Its Related Statements]]