
## Synthesis
- 
## Examples [^1]
### Factoring Trinomial with 2 Variables
- $$ \begin{align*} 8x^2 - 6xy - 9y^2 &&\text{Given} \\8x^2 \textcolor{hotpink}{- 12xy + 6xy} - 9y^2 && \text{Find factors of \textcolor{red}{ac} and addends of \textcolor{red}{b}} \\ 4x(2x-3y) + 3y(2x-3y) && \text{Factor out terms} \\(4x +3y)(2x-3y) &&\text{Factor by grouping} \end{align*}  $$
## Personal
### Shortcut Method #1 (Divide by x Term)
- $$ \begin{align*} 8x^2 - 6xy -9y^2 && \text{Given} \\ \textcolor{hotpink}{-12xy \text{ and }6xy} \text{ are factors of ac that work} && \text{Find factors} \\\frac{-12xy}{8x^2} \to \frac{-3y}{2x} \to (2x -3y) &&\text{Divide by x term} \\\frac{6xy}{8x^2} \to \frac{3y}{4x} \to (4x +3y) \\(2x-3y)(4x+3y) && \text{Solution} \end{align*}  $$
### Shortcut Method #2 (Divide by y Term)
- $$ \begin{align*} 8x^2 - 6xy -9y^2 && \text{Given} \\ \textcolor{hotpink}{-12xy \text{ and }6xy} \text{ are factors of ac that work} && \text{Find factors} \\\frac{-12xy}{-9y^2} \to \frac{4x}{3y} \to (3y +4x) &&\text{Divide by y term} \\\frac{6xy}{-9y^2} \to \frac{2x}{-3y} \to (-3y +2x) \\(2x-3y)(4x+3y) && \text{Solution} \end{align*}  $$
## References
[^1]: [[(Video) Factoring an expression with a greater than one and two square variables 8x squared -6xy -9y squared]]