## Synthesis

## Source [^1]
### Example

- Given 
	- A = $\begin{bmatrix}2 & 1\\ 5 & 3\end{bmatrix}$
- Formulas 
	- A = $\begin{bmatrix}a & b\\ c & d\end{bmatrix}$
	- $A^{-1}$ = $\frac {1}{(ad-bc)}\begin{bmatrix}d & -b\\ -c & a\end{bmatrix}$ 
- Solving
	- $A^{-1}$ = $\frac {1}{(2)(3)-(1)(5)}\begin{bmatrix}3 & -1\\ -5 & 2\end{bmatrix}$ (scalar multiplying a matrix)
- Solution
	- $A^{-1}$ = $\begin{bmatrix}3 & -1\\ -5 & 2\end{bmatrix}$
## References

[^1]: [[(22) PreCalculus - Matrices & Matrix Applications (21 of 33) Using the Determinant to Find the Inverse]]